field_compat

floyd/field_compat.v
@@ -11,6 +11,8 @@ Require Import VST.floyd.jmeq_lemmas.
 Require Import VST.zlist.sublist.
 Require Import VST.floyd.field_at.
 
+Local Unset SsrRewrite.
+
 Lemma field_compatible_offset_zero:
   forall {cs: compspecs} t gfs p,
     field_compatible t gfs p <-> field_compatible t gfs (offset_val 0 p).
@@ -263,25 +265,29 @@ Qed.
 #[export] Hint Extern 2 (field_compatible0 _ _ (offset_val _ _)) =>
   (apply field_compatible0_nested_field_array; auto with field_compatible) : core. (*FIXME: should be field_compatible*)
 
+Section mpred.
+
+Context `{!heapGS Σ}.
+
 Lemma split2_data_at_Tarray_unfold {cs: compspecs}
      sh t n n1 (v v' v1 v2: list (reptype t)) p:
    0 <= n1 <= n ->
   v = v' ->
   v1 = (sublist 0 n1 v') ->
   v2 = (sublist n1 n v') ->
-  data_at sh (Tarray t n noattr) v p |--
-  data_at sh (Tarray t n1 noattr) v1 p *
+  data_at sh (Tarray t n noattr) v p ⊢
+  data_at sh (Tarray t n1 noattr) v1 p ∗
   data_at sh (Tarray t (n - n1) noattr) v2
     (field_address0 (Tarray t n noattr) (ArraySubsc n1::nil) p).
 Proof.
   intros.
   assert_PROP (Zlength v' = n). {
-    eapply derives_trans; [apply data_at_local_facts | apply prop_derives].
+    rewrite data_at_local_facts; apply bi.pure_mono.
     intros [? ?]. destruct H4 as [? _]. rewrite Z.max_r in H4 by lia.
     rewrite <- H0. exact H4.
   }
   assert_PROP (field_compatible0 (Tarray t n noattr) (ArraySubsc n1::nil) p). {
-     eapply derives_trans; [apply data_at_local_facts | apply prop_derives].
+    rewrite data_at_local_facts; apply bi.pure_mono.
      intros [? _]; auto with field_compatible.
   }
   rewrite field_address0_offset by auto.
@@ -321,55 +327,46 @@ Lemma split2_data_at_Tarray_fold {cs: compspecs} sh t n n1 (v v' v1 v2: list (re
    v = (sublist 0 n v') ->
    v1 = (sublist 0 n1 v') ->
    v2 = (sublist n1 n v') ->
-   data_at sh (Tarray t n1 noattr) v1 p *
+   data_at sh (Tarray t n1 noattr) v1 p ∗
    data_at sh (Tarray t (n - n1) noattr) v2
         (field_address0 (Tarray t n noattr) (ArraySubsc n1::nil) p)
-   |--
+   ⊢
    data_at sh (Tarray t n noattr) v p.
 Proof.
   intros until 1. intro Hn; intros.
   unfold field_address0.
-  if_tac; [ |
-  eapply derives_trans; [apply sepcon_derives;
-           apply prop_and_same_derives; apply data_at_local_facts
-    | normalize ];
-  destruct H6; contradiction].
+  if_tac; [| iIntros "(? & H)"; iDestruct (data_at_local_facts with "H") as %((? & ?) & ?); contradiction].
   assert_PROP (field_compatible (Tarray t n noattr) nil p). {
-    eapply derives_trans.
-    apply sepcon_derives; apply prop_and_same_derives; apply data_at_local_facts .
-    normalize. apply prop_right.
-   clear - H3 H4 H.
-   hnf in H3,H4|-*; intuition.
+    iIntros "(? & H)"; iDestruct (data_at_local_facts with "H") as %(H4 & _).
+    clear - H3 H4 H; iPureIntro.
+    hnf in H3,H4|-*; intuition.
   } clear H3; rename H4 into H3.
   rewrite data_at_isptr at 1. unfold at_offset. intros; normalize.
-  unfold data_at at 3.  erewrite field_at_Tarray; try reflexivity; eauto; try lia.
+  unfold data_at at 3. erewrite field_at_Tarray; try reflexivity; eauto; try lia.
   rewrite H0.
   rewrite (split2_array_at sh (Tarray t n noattr) nil 0 n1); trivial.
   2: autorewrite with sublist; auto.
   autorewrite with sublist.
   unfold data_at at 1; erewrite field_at_Tarray; try reflexivity; eauto; try lia.
   unfold data_at at 1; erewrite field_at_Tarray; try reflexivity; eauto; try lia.
-  apply sepcon_derives.
+  apply bi.sep_mono.
   unfold array_at.
   rewrite H1.
-  simpl. apply andp_derives; auto.
-  2: apply derives_refl. 
-  apply prop_derives. intuition auto with field_compatible.
+  simpl. apply bi.and_mono; auto.
+  { apply bi.pure_mono. intuition auto with field_compatible. }
   assert (sublist n1 (Z.min n (Zlength v')) v' = sublist n1 n v').
-  f_equal. autorewrite with sublist. auto.
+  { f_equal. autorewrite with sublist. auto. }
   rewrite H2.
   clear - H H3.
   rewrite array_at_data_at by lia. normalize.
   rewrite array_at_data_at by lia.
   rewrite !prop_true_andp by auto with field_compatible.
   unfold at_offset.
-  apply derives_refl'.
   rewrite offset_offset_val.
   rewrite !nested_field_offset_ind by (repeat split; auto; lia).
   rewrite !nested_field_type_ind. unfold gfield_offset.
   rewrite !Z.add_0_l. rewrite Z.mul_0_r, Z.add_0_r.
-  apply equal_f.
-  apply data_at_type_changable; auto.
+  erewrite data_at_type_changable; auto.
   unfold nested_field_array_type.
   rewrite !nested_field_type_ind.  unfold gfield_type. simpl. f_equal; lia.
 Qed.
@@ -380,15 +377,16 @@ Lemma split2_data_at_Tarray {cs: compspecs} sh t n n1 (v v' v1 v2: list (reptype
    v = (sublist 0 n v') ->
    v1 = (sublist 0 n1 v') ->
    v2 = (sublist n1 n v') ->
-   data_at sh (Tarray t n noattr) v p =
-    data_at sh (Tarray t n1 noattr) v1 p *
+   data_at sh (Tarray t n noattr) v p ⊣⊢
+    data_at sh (Tarray t n1 noattr) v1 p ∗
     data_at sh (Tarray t (n - n1) noattr) v2 (field_address0 (Tarray t n noattr) (ArraySubsc n1::nil) p).
-Proof. intros.
- apply pred_ext.
- eapply split2_data_at_Tarray_unfold; try eassumption.
-  autorewrite with sublist; auto.
-  autorewrite with sublist; auto.
- eapply split2_data_at_Tarray_fold; try eassumption.
+Proof.
+  intros.
+  apply bi.equiv_entails_2.
+  - eapply split2_data_at_Tarray_unfold; try eassumption.
+    autorewrite with sublist; auto.
+    autorewrite with sublist; auto.
+  - eapply split2_data_at_Tarray_fold; try eassumption.
 Qed.
 
 Lemma field_compatible0_Tarray_offset:
@@ -402,7 +400,7 @@ Lemma field_compatible0_Tarray_offset:
   p' = offset_val (sizeof t * (i'-i)) p ->
   field_compatible0 (Tarray t n noattr) (ArraySubsc i :: nil) p'.
 Proof.
-intros until 1. intros NA ?H ?H Hni Hii Hp. subst p'.
+  intros until 1. intros NA ?H ?H Hni Hii Hp. subst p'.
   assert (SP := sizeof_pos t).
   assert (SS: sizeof t * n <= sizeof t * n').
   apply Zmult_le_compat_l. lia. lia.
@@ -469,11 +467,12 @@ Lemma split3_data_at_Tarray {cs: compspecs} sh t n n1 n2 v (v' v1 v2 v3: list (r
    v1 = (sublist 0 n1 v') ->
    v2 = (sublist n1 n2 v') ->
    v3 = (sublist n2 n v') ->
-   data_at sh (Tarray t n noattr) v p =
-    data_at sh (Tarray t n1 noattr) v1 p *
-    data_at sh (Tarray t (n2 - n1) noattr) v2 (field_address0 (Tarray t n noattr) (ArraySubsc n1::nil) p) *
+   data_at sh (Tarray t n noattr) v p ⊣⊢
+    data_at sh (Tarray t n1 noattr) v1 p ∗
+    data_at sh (Tarray t (n2 - n1) noattr) v2 (field_address0 (Tarray t n noattr) (ArraySubsc n1::nil) p) ∗
     data_at sh (Tarray t (n - n2) noattr) v3 (field_address0 (Tarray t n noattr) (ArraySubsc n2::nil) p).
-Proof. intros until 1. rename H into NA; intros.
+Proof.
+  intros until 1. rename H into NA; intros.
   destruct (field_compatible0_dec (tarray t n) (ArraySubsc n2::nil) p).
   erewrite (split2_data_at_Tarray sh t n n1); try eassumption; try lia.
   instantiate (1:= sublist n1 n v').
@@ -487,14 +486,12 @@ Proof. intros until 1. rename H into NA; intros.
   2: autorewrite with sublist;
      instantiate (1:= sublist n2 n v');
      auto.
-  rewrite sepcon_assoc.
-  f_equal. f_equal. f_equal. auto.
+  f_equiv. f_equiv. f_equiv. auto.
   replace  (field_address0 (Tarray t (n - n1) noattr) (SUB (n2 - n1))
      (field_address0 (Tarray t n noattr) (SUB n1) p))
    with (field_address0 (Tarray t n noattr) (SUB n2) p).
-  apply equal_f.
-  replace (n - n1 - (n2 - n1)) with (n - n2) by lia.
-  subst v3; reflexivity.
+  { replace (n - n1 - (n2 - n1)) with (n - n2) by lia.
+    subst v3; reflexivity. }
   rewrite field_address0_offset by auto with field_compatible.
   rewrite (field_address0_offset (Tarray t n noattr) ) by auto with field_compatible.
   rewrite field_address0_offset.
@@ -508,89 +505,93 @@ Proof. intros until 1. rename H into NA; intros.
   rewrite Z.add_0_l.
   eapply field_compatible0_Tarray_offset; try eassumption; try lia.
   f_equal. f_equal. lia.
-  apply pred_ext.
-  eapply derives_trans. apply data_at_local_facts. normalize.
+  apply bi.equiv_entails_2.
+  iIntros "H"; iDestruct (data_at_local_facts with "H") as %(? & ?).
   contradiction n0. auto with field_compatible.
   unfold field_address0 at 2.
   if_tac.
   contradiction n0. auto with field_compatible.
-  eapply derives_trans. apply sepcon_derives; [apply derives_refl | ].
-  apply prop_and_same_derives; apply data_at_local_facts .
-  normalize. destruct H6 as [H6 _]; contradiction H6.
+  iIntros "(? & ? & H)"; iDestruct (data_at_local_facts with "H") as %((? & ?) & ?).
+  contradiction.
 Qed.
 
 Lemma split2_data_at_Tarray_tuchar {cs: compspecs} sh n n1 (v: list val) p:
    0 <= n1 <= n ->
    Zlength v = n ->
-   data_at sh (Tarray tuchar n noattr) v p =
-    data_at sh (Tarray tuchar n1 noattr) (sublist 0 n1 v) p *
+   data_at sh (Tarray tuchar n noattr) v p ⊣⊢
+    data_at sh (Tarray tuchar n1 noattr) (sublist 0 n1 v) p ∗
     data_at sh (Tarray tuchar (n - n1) noattr) (sublist n1 n v) (field_address0 (Tarray tuchar n noattr) (ArraySubsc n1::nil) p).
-Proof. intros.
- eapply split2_data_at_Tarray; auto;
- change (@reptype cs tuchar) with val.
- symmetry in H0.
- list_solve.
- rewrite sublist_same; try lia; auto.
+Proof.
+  intros.
+  eapply split2_data_at_Tarray; auto;
+  change (@reptype cs tuchar) with val.
+  symmetry in H0.
+  list_solve.
+  rewrite sublist_same; try lia; auto.
 Qed.
 
 Lemma split2_data_at_Tarray_tschar {cs: compspecs} sh n n1 (v: list val) p:
    0 <= n1 <= n ->
    Zlength v = n ->
-   data_at sh (Tarray tschar n noattr) v p =
-    data_at sh (Tarray tschar n1 noattr) (sublist 0 n1 v) p *
+   data_at sh (Tarray tschar n noattr) v p ⊣⊢
+    data_at sh (Tarray tschar n1 noattr) (sublist 0 n1 v) p ∗
     data_at sh (Tarray tschar (n - n1) noattr) (sublist n1 n v) (field_address0 (Tarray tschar n noattr) (ArraySubsc n1::nil) p).
-Proof. intros.
- eapply split2_data_at_Tarray; auto;
- change (@reptype cs tschar) with val.
- symmetry in H0.
- list_solve.
- rewrite sublist_same; try lia; auto.
+Proof.
+  intros.
+  eapply split2_data_at_Tarray; auto;
+  change (@reptype cs tschar) with val.
+  symmetry in H0.
+  list_solve.
+  rewrite sublist_same; try lia; auto.
 Qed.
 
 Lemma split3_data_at_Tarray_tuchar {cs: compspecs} sh n n1 n2 (v: list val) p:
    0 <= n1 <= n2 ->
    n2 <= n ->
    Zlength v = n ->
-   data_at sh (Tarray tuchar n noattr) v p =
-    data_at sh (Tarray tuchar n1 noattr) (sublist 0 n1 v) p *
-    data_at sh (Tarray tuchar (n2 - n1) noattr) (sublist n1 n2 v) (field_address0 (Tarray tuchar n noattr) (ArraySubsc n1::nil) p) *
+   data_at sh (Tarray tuchar n noattr) v p ⊣⊢
+    data_at sh (Tarray tuchar n1 noattr) (sublist 0 n1 v) p ∗
+    data_at sh (Tarray tuchar (n2 - n1) noattr) (sublist n1 n2 v) (field_address0 (Tarray tuchar n noattr) (ArraySubsc n1::nil) p) ∗
     data_at sh (Tarray tuchar (n - n2) noattr) (sublist n2 n v) (field_address0 (Tarray tuchar n noattr) (ArraySubsc n2::nil) p).
-Proof. intros.
- eapply split3_data_at_Tarray; auto;
- change (@reptype cs tuchar) with val.
+Proof.
+  intros.
+  eapply split3_data_at_Tarray; auto;
+  change (@reptype cs tuchar) with val.
   split; simpl; auto. list_solve.
- rewrite sublist_same; try lia; auto.
+  rewrite sublist_same; try lia; auto.
 Qed.
 
 Lemma split3_data_at_Tarray_tschar {cs: compspecs} sh n n1 n2 (v: list val) p:
    0 <= n1 <= n2 ->
    n2 <= n ->
    Zlength v = n ->
-   data_at sh (Tarray tschar n noattr) v p =
-    data_at sh (Tarray tschar n1 noattr) (sublist 0 n1 v) p *
-    data_at sh (Tarray tschar (n2 - n1) noattr) (sublist n1 n2 v) (field_address0 (Tarray tschar n noattr) (ArraySubsc n1::nil) p) *
+   data_at sh (Tarray tschar n noattr) v p ⊣⊢
+    data_at sh (Tarray tschar n1 noattr) (sublist 0 n1 v) p ∗
+    data_at sh (Tarray tschar (n2 - n1) noattr) (sublist n1 n2 v) (field_address0 (Tarray tschar n noattr) (ArraySubsc n1::nil) p) ∗
     data_at sh (Tarray tschar (n - n2) noattr) (sublist n2 n v) (field_address0 (Tarray tschar n noattr) (ArraySubsc n2::nil) p).
-Proof. intros.
- eapply split3_data_at_Tarray; auto;
- change (@reptype cs tschar) with val.
+Proof.
+  intros.
+  eapply split3_data_at_Tarray; auto;
+  change (@reptype cs tschar) with val.
   split; simpl; auto. list_solve.
- rewrite sublist_same; try lia; auto.
+  rewrite sublist_same; try lia; auto.
 Qed.
 
-Lemma sizeof_tarray_tuchar {cs} n (N:0<=n): @sizeof cs (tarray tuchar n) = n.
+Lemma sizeof_tarray_tuchar {cs : compspecs} n (N:0<=n): @sizeof cs (tarray tuchar n) = n.
 Proof. unfold sizeof; simpl. rewrite Z.max_r. destruct n; trivial. lia. Qed. 
 
-Lemma sizeof_tarray_tschar {cs} n (N:0<=n): @sizeof cs (tarray tschar n) = n.
+Lemma sizeof_tarray_tschar {cs : compspecs} n (N:0<=n): @sizeof cs (tarray tschar n) = n.
 Proof. unfold sizeof; simpl. rewrite Z.max_r. destruct n; trivial. lia. Qed. 
 
 Opaque sizeof.
 Import ListNotations.
 
-Lemma memory_block_field_compatible_tarraytuchar_ent {cs} sh n p (N:0<=n < Ptrofs.modulus):
-memory_block sh n p |-- !! @field_compatible cs (tarray tuchar n) nil p.
-Proof. Transparent memory_block. unfold memory_block. Opaque memory_block.
-   destruct p; try solve [apply FF_left]. normalize.
-   apply prop_right. red.
+Lemma memory_block_field_compatible_tarraytuchar_ent {cs : compspecs} sh n p (N:0<=n < Ptrofs.modulus):
+memory_block sh n p ⊢ ⌜@field_compatible cs (tarray tuchar n) nil p⌝.
+Proof.
+  Transparent memory_block. unfold memory_block. Opaque memory_block.
+   destruct p; try solve [iIntros "[]"]. normalize.
+   apply bi.pure_intro. red.
    destruct (Ptrofs.unsigned_range i). simpl.
    repeat split; try rewrite sizeof_tarray_tuchar; trivial; try lia.
    (* TODO: abstract this proof. *)
@@ -603,11 +604,12 @@ Proof. Transparent memory_block. unfold memory_block. Opaque memory_block.
    + reflexivity.
 Qed.
 
-Lemma memory_block_field_compatible_tarraytschar_ent {cs} sh n p (N:0<=n < Ptrofs.modulus):
-memory_block sh n p |-- !! @field_compatible cs (tarray tschar n) nil p.
-Proof. Transparent memory_block. unfold memory_block. Opaque memory_block.
-   destruct p; try solve [apply FF_left]. normalize.
-   apply prop_right. red.
+Lemma memory_block_field_compatible_tarraytschar_ent {cs : compspecs} sh n p (N:0<=n < Ptrofs.modulus):
+memory_block sh n p ⊢ ⌜@field_compatible cs (tarray tschar n) nil p⌝.
+Proof.
+  Transparent memory_block. unfold memory_block. Opaque memory_block.
+   destruct p; try solve [iIntros "[]"]. normalize.
+   apply bi.pure_intro. red.
    destruct (Ptrofs.unsigned_range i). simpl.
    repeat split; try rewrite sizeof_tarray_tschar; trivial; try lia.
    (* TODO: abstract this proof. *)
@@ -620,22 +622,22 @@ Proof. Transparent memory_block. unfold memory_block. Opaque memory_block.
    + reflexivity.
 Qed.
 
-Lemma memory_block_field_compatible_tarraytuchar {cs} sh n p (N:0<=n < Ptrofs.modulus):
-memory_block sh n p = !!(@field_compatible cs (tarray tuchar n) nil p) && memory_block sh n p.
-Proof. apply pred_ext. apply andp_right; trivial. apply memory_block_field_compatible_tarraytuchar_ent; trivial.
+Lemma memory_block_field_compatible_tarraytuchar {cs : compspecs} sh n p (N:0<=n < Ptrofs.modulus):
+memory_block sh n p ⊣⊢ ⌜@field_compatible cs (tarray tuchar n) nil p⌝ ∧ memory_block sh n p.
+Proof. apply bi.equiv_entails_2. apply bi.and_intro; trivial. apply memory_block_field_compatible_tarraytuchar_ent; trivial.
 normalize.
 Qed. 
 
-Lemma memory_block_field_compatible_tarraytschar {cs} sh n p (N:0<=n < Ptrofs.modulus):
-memory_block sh n p = !!(@field_compatible cs (tarray tschar n) nil p) && memory_block sh n p.
-Proof. apply pred_ext. apply andp_right; trivial. apply memory_block_field_compatible_tarraytschar_ent; trivial.
+Lemma memory_block_field_compatible_tarraytschar {cs : compspecs} sh n p (N:0<=n < Ptrofs.modulus):
+memory_block sh n p ⊣⊢ ⌜@field_compatible cs (tarray tschar n) nil p⌝ ∧ memory_block sh n p.
+Proof. apply bi.equiv_entails_2. apply bi.and_intro; trivial. apply memory_block_field_compatible_tarraytschar_ent; trivial.
 normalize.
 Qed. 
 
-Lemma memory_block_data_at__tarray_tuchar {cs} sh p n (N: 0<=n < Ptrofs.modulus):
-  memory_block sh n p |-- @data_at_ cs sh (tarray tuchar n) p.
+Lemma memory_block_data_at__tarray_tuchar {cs : compspecs} sh p n (N: 0<=n < Ptrofs.modulus):
+  memory_block sh n p ⊢ data_at_ sh (tarray tuchar n) p.
 Proof. 
-  rewrite memory_block_field_compatible_tarraytuchar, memory_block_isptr; trivial. 
+  rewrite memory_block_field_compatible_tarraytuchar, memory_block_isptr; trivial.
   normalize. destruct p; try solve [inv Pp].
   unfold data_at_, data_at.
   rewrite field_at__memory_block. 
@@ -644,38 +646,38 @@ Proof.
   rewrite Ptrofs.add_zero, sizeof_tarray_tuchar; try apply derives_refl; lia.
 Qed.
 
-Lemma memory_block_data_at__tarray_tschar {cs} sh p n (N: 0<=n < Ptrofs.modulus):
-  memory_block sh n p |-- @data_at_ cs sh (tarray tschar n) p.
+Lemma memory_block_data_at__tarray_tschar {cs : compspecs} sh p n (N: 0<=n < Ptrofs.modulus):
+  memory_block sh n p ⊢ data_at_ sh (tarray tschar n) p.
 Proof. 
-  rewrite memory_block_field_compatible_tarraytschar, memory_block_isptr; trivial. 
+  rewrite memory_block_field_compatible_tarraytschar, memory_block_isptr; trivial.
   normalize. destruct p; try solve [inv Pp].
   unfold data_at_, data_at.
-  rewrite field_at__memory_block. 
+  rewrite field_at__memory_block.
   unfold field_address. rewrite if_true; trivial.
   unfold nested_field_offset, nested_field_type; simpl.
   rewrite Ptrofs.add_zero, sizeof_tarray_tschar; try apply derives_refl; lia.
 Qed.
 
-Lemma memory_block_data_at__tarray_tuchar_eq {cs} sh p n (N: 0<=n < Ptrofs.modulus):
-  memory_block sh n p = @data_at_ cs sh (tarray tuchar n) p.
+Lemma memory_block_data_at__tarray_tuchar_eq {cs : compspecs} sh p n (N: 0<=n < Ptrofs.modulus):
+  memory_block sh n p ⊣⊢ data_at_ sh (tarray tuchar n) p.
 Proof.
-  apply pred_ext. apply memory_block_data_at__tarray_tuchar; trivial.
-  rewrite data_at__memory_block; simpl. normalize. 
-  rewrite sizeof_tarray_tuchar; try apply derives_refl; lia. 
+  apply bi.equiv_entails_2. apply memory_block_data_at__tarray_tuchar; trivial.
+  rewrite data_at__memory_block; simpl. normalize.
+  rewrite sizeof_tarray_tuchar; try apply derives_refl; lia.
 Qed.
 
-Lemma memory_block_data_at__tarray_tschar_eq {cs} sh p n (N: 0<=n < Ptrofs.modulus):
-  memory_block sh n p = @data_at_ cs sh (tarray tschar n) p.
+Lemma memory_block_data_at__tarray_tschar_eq {cs : compspecs} sh p n (N: 0<=n < Ptrofs.modulus):
+  memory_block sh n p ⊣⊢ data_at_ sh (tarray tschar n) p.
 Proof.
-  apply pred_ext. apply memory_block_data_at__tarray_tschar; trivial.
+  apply bi.equiv_entails_2. apply memory_block_data_at__tarray_tschar; trivial.
   rewrite data_at__memory_block; simpl. normalize. 
   rewrite sizeof_tarray_tschar; try apply derives_refl; lia. 
 Qed.
 
-Lemma isptr_field_compatible0_tarray {cs}:
+Lemma isptr_field_compatible0_tarray {cs : compspecs}:
   forall t (H: complete_legal_cosu_type t = true) p,
        isptr p -> 
-      @field_compatible cs (tarray t 0) nil p.
+      field_compatible (tarray t 0) nil p.
 Proof. intros; red. destruct p; try contradiction.
   repeat split; simpl; trivial.
   change (sizeof (tarray t 0)) with (sizeof t * 0)%Z.
@@ -686,14 +688,14 @@ Qed.
 
 Transparent sizeof.
 
-Lemma data_at_singleton_array {cs} sh t vl v p:
+Lemma data_at_singleton_array {cs : compspecs} sh t vl v p:
   vl = [v] ->
-  @data_at cs sh t v p |-- @data_at cs sh (tarray t 1) vl p.  
+  data_at sh t v p ⊢ data_at sh (tarray t 1) vl p.  
 Proof.
   intros. rename H into Heq.
   rewrite data_at_isptr. normalize.
   assert_PROP (field_compatible (tarray t 1) [] p).
-  { eapply derives_trans. eapply data_at_local_facts. normalize.
+  { iIntros "H"; iDestruct (data_at_local_facts with "H") as %(? & ?); iPureIntro.
     destruct p; auto.
     inv_int i.
     destruct H as [? [? [? [? ?]]]].
@@ -716,13 +718,13 @@ Proof.
   eapply field_compatible_cons_Tarray. reflexivity. trivial. lia.
 Qed.
 
-Lemma data_at_singleton_array_inv {cs} sh t (vl : list (reptype t)) v p:
+Lemma data_at_singleton_array_inv {cs : compspecs} sh t (vl : list (reptype t)) v p:
   vl = [v] ->
-  @data_at cs sh (tarray t 1) vl p |-- @data_at cs sh t v p.  
+  data_at sh (tarray t 1) vl p ⊢ data_at sh t v p.
 Proof.
   rewrite data_at_isptr. normalize.
   assert_PROP (field_compatible (tarray t 1) [] p).
-  { eapply derives_trans. eapply data_at_local_facts. normalize. }
+  { rewrite data_at_local_facts; apply bi.pure_mono; tauto. }
   unfold data_at at 1.
   erewrite field_at_Tarray.
   2: simpl; trivial. 2: reflexivity. 2: lia. 2: apply JMeq_refl.
@@ -736,62 +738,62 @@ Proof.
 Qed.
 
 Opaque sizeof.
- 
-Lemma data_at_singleton_array_eq {cs} sh t v (vl: list (reptype t)) p:
+
+Lemma data_at_singleton_array_eq {cs : compspecs} sh t v (vl: list (reptype t)) p:
   vl = [v] ->
-  @data_at cs sh (tarray t 1) vl p = @data_at cs sh t v p.  
+  data_at sh (tarray t 1) vl p ⊣⊢ data_at sh t v p.
 Proof. 
   intros.
-   apply pred_ext.
+   apply bi.equiv_entails_2.
   apply data_at_singleton_array_inv; rewrite H; auto.
   apply data_at_singleton_array; auto.
 Qed.
 
-Lemma data_at_tuchar_singleton_array {cs} sh (v: val) p:
-  @data_at cs sh tuchar v p |-- @data_at cs sh (tarray tuchar 1) [v] p.  
+Lemma data_at_tuchar_singleton_array {cs : compspecs} sh (v: val) p:
+  data_at sh tuchar v p ⊢ data_at sh (tarray tuchar 1) [v] p.  
 Proof. apply data_at_singleton_array. reflexivity. Qed.
 
-Lemma data_at_tschar_singleton_array {cs} sh (v: val) p:
-  @data_at cs sh tschar v p |-- @data_at cs sh (tarray tschar 1) [v] p.  
+Lemma data_at_tschar_singleton_array {cs : compspecs} sh (v: val) p:
+  data_at sh tschar v p ⊢ data_at sh (tarray tschar 1) [v] p.  
 Proof. apply data_at_singleton_array. reflexivity. Qed.
 
-Lemma data_at_tuchar_singleton_array_inv {cs} sh (v: val) p:
-  @data_at cs sh (tarray tuchar 1) [v] p |-- @data_at cs sh tuchar v p.  
+Lemma data_at_tuchar_singleton_array_inv {cs : compspecs} sh (v: val) p:
+  data_at sh (tarray tuchar 1) [v] p ⊢ data_at sh tuchar v p.  
 Proof. apply data_at_singleton_array_inv. reflexivity. Qed.
 
-Lemma data_at_tschar_singleton_array_inv {cs} sh (v: val) p:
-  @data_at cs sh (tarray tschar 1) [v] p |-- @data_at cs sh tschar v p.  
+Lemma data_at_tschar_singleton_array_inv {cs : compspecs} sh (v: val) p:
+  data_at sh (tarray tschar 1) [v] p ⊢ data_at sh tschar v p.  
 Proof. apply data_at_singleton_array_inv. reflexivity. Qed.
 
-Lemma data_at_tuchar_singleton_array_eq {cs} sh (v: val) p:
-  @data_at cs sh (tarray tuchar 1) [v] p = @data_at cs sh tuchar v p.  
+Lemma data_at_tuchar_singleton_array_eq {cs : compspecs} sh (v: val) p:
+  data_at sh (tarray tuchar 1) [v] p ⊣⊢ data_at sh tuchar v p.  
 Proof. apply data_at_singleton_array_eq. reflexivity. Qed.
 
-Lemma data_at_tschar_singleton_array_eq {cs} sh (v: val) p:
-  @data_at cs sh (tarray tschar 1) [v] p = @data_at cs sh tschar v p.  
+Lemma data_at_tschar_singleton_array_eq {cs : compspecs} sh (v: val) p:
+  data_at sh (tarray tschar 1) [v] p ⊣⊢ data_at sh tschar v p.  
 Proof. apply data_at_singleton_array_eq. reflexivity. Qed.
 
-Lemma data_at_zero_array {cs} sh t (v: list (reptype t)) p:
+Lemma data_at_zero_array {cs : compspecs} sh t (v: list (reptype t)) p:
   complete_legal_cosu_type t = true ->
   isptr p ->
   v = (@nil (reptype t)) ->
-  emp |-- @data_at cs sh (tarray t 0) v p.  
+  emp ⊢ data_at sh (tarray t 0) v p.  
 Proof. intros.
   unfold data_at. 
   erewrite field_at_Tarray. 3: reflexivity. 3: lia. 3: apply JMeq_refl. 2: simpl; trivial.
   rewrite H1.
-  rewrite array_at_len_0. apply andp_right; try apply derives_refl.
-  apply prop_right.
+  rewrite array_at_len_0. apply bi.and_intro; try apply derives_refl.
+  apply bi.pure_intro.
   apply field_compatible0_ArraySubsc0.
   apply isptr_field_compatible0_tarray; auto.
  simpl.
   split; auto. lia.
 Qed.
 
-Lemma data_at_zero_array_inv {cs} sh t (v: list (reptype t)) p:
+Lemma data_at_zero_array_inv {cs : compspecs} sh t (v: list (reptype t)) p:
   complete_legal_cosu_type t = true ->
   v = (@nil (reptype t)) ->
-  @data_at cs sh (tarray t 0) v p |-- emp.  
+  data_at sh (tarray t 0) v p ⊢ emp.  
 Proof. intros.
   unfold data_at. 
   erewrite field_at_Tarray. 3: reflexivity. 3: lia. 3: rewrite H0; apply JMeq_refl. 2: simpl; trivial.
@@ -799,83 +801,84 @@ Proof. intros.
   rewrite array_at_len_0. normalize. 
 Qed.
 
-Lemma data_at_zero_array_eq {cs} sh t (v: list (reptype t)) p:
+Lemma data_at_zero_array_eq {cs : compspecs} sh t (v: list (reptype t)) p:
   complete_legal_cosu_type t = true ->
   isptr p ->
   v = (@nil (reptype t)) ->
-  @data_at cs sh (tarray t 0) v p = emp.
+  data_at sh (tarray t 0) v p ⊣⊢ emp.
 Proof. intros. 
-  apply pred_ext.
+  apply bi.equiv_entails_2.
   apply data_at_zero_array_inv; auto.
   apply data_at_zero_array; auto.
 Qed. 
 
-Lemma data_at_tuchar_zero_array {cs} sh p: isptr p ->
-  emp |-- @data_at cs sh (tarray tuchar 0) [] p.  
+Lemma data_at_tuchar_zero_array {cs : compspecs} sh p: isptr p ->
+  emp ⊢ data_at sh (tarray tuchar 0) [] p.  
 Proof. intros. apply data_at_zero_array; auto. Qed.
 
-Lemma data_at_tschar_zero_array {cs} sh p: isptr p ->
-  emp |-- @data_at cs sh (tarray tschar 0) [] p.  
+Lemma data_at_tschar_zero_array {cs : compspecs} sh p: isptr p ->
+  emp ⊢ data_at sh (tarray tschar 0) [] p.  
 Proof. intros. apply data_at_zero_array; auto. Qed.
 
-Lemma data_at_tuchar_zero_array_inv {cs} sh p:
-  @data_at cs sh (tarray tuchar 0) [] p |-- emp.  
+Lemma data_at_tuchar_zero_array_inv {cs : compspecs} sh p:
+  data_at sh (tarray tuchar 0) [] p ⊢ emp.  
 Proof. intros. apply data_at_zero_array_inv; auto. Qed.
 
-Lemma data_at_tschar_zero_array_inv {cs} sh p:
-  @data_at cs sh (tarray tschar 0) [] p |-- emp.  
+Lemma data_at_tschar_zero_array_inv {cs : compspecs} sh p:
+  data_at sh (tarray tschar 0) [] p ⊢ emp.  
 Proof. intros. apply data_at_zero_array_inv; auto. Qed.
 
-Lemma data_at_tuchar_zero_array_eq {cs} sh p:
+Lemma data_at_tuchar_zero_array_eq {cs : compspecs} sh p:
   isptr p ->
-  @data_at cs sh (tarray tuchar 0) [] p = emp.  
+  data_at sh (tarray tuchar 0) [] p ⊣⊢ emp.  
 Proof. intros. apply data_at_zero_array_eq; auto. Qed.
 
-Lemma data_at_tschar_zero_array_eq {cs} sh p:
+Lemma data_at_tschar_zero_array_eq {cs : compspecs} sh p:
   isptr p ->
-  @data_at cs sh (tarray tschar 0) [] p = emp.  
+  data_at sh (tarray tschar 0) [] p ⊣⊢ emp.  
 Proof. intros. apply data_at_zero_array_eq; auto. Qed.
 
-Lemma data_at__tuchar_zero_array {cs} sh p (H: isptr p):
-  emp |-- @data_at_ cs sh (tarray tuchar 0) p.  
+Lemma data_at__tuchar_zero_array {cs : compspecs} sh p (H: isptr p):
+  emp ⊢ data_at_ sh (tarray tuchar 0) p.  
 Proof. unfold data_at_, field_at_. apply data_at_tuchar_zero_array; trivial. Qed.
 
-Lemma data_at__tschar_zero_array {cs} sh p (H: isptr p):
-  emp |-- @data_at_ cs sh (tarray tschar 0) p.  
+Lemma data_at__tschar_zero_array {cs : compspecs} sh p (H: isptr p):
+  emp ⊢ data_at_ sh (tarray tschar 0) p.  
 Proof. unfold data_at_, field_at_. apply data_at_tschar_zero_array; trivial. Qed.
 
-Lemma data_at__tuchar_zero_array_inv {cs} sh p:
-  @data_at_ cs sh (tarray tuchar 0) p |-- emp.  
+Lemma data_at__tuchar_zero_array_inv {cs : compspecs} sh p:
+  data_at_ sh (tarray tuchar 0) p ⊢ emp.  
 Proof. unfold data_at_, field_at_. apply data_at_tuchar_zero_array_inv. Qed.
 
-Lemma data_at__tschar_zero_array_inv {cs} sh p:
-  @data_at_ cs sh (tarray tschar 0) p |-- emp.  
+Lemma data_at__tschar_zero_array_inv {cs : compspecs} sh p:
+  data_at_ sh (tarray tschar 0) p ⊢ emp.  
 Proof. unfold data_at_, field_at_. apply data_at_tschar_zero_array_inv. Qed.
 
-Lemma data_at__tuchar_zero_array_eq {cs} sh p (H: isptr p):
-  @data_at_ cs sh (tarray tuchar 0) p = emp.  
+Lemma data_at__tuchar_zero_array_eq {cs : compspecs} sh p (H: isptr p):
+  data_at_ sh (tarray tuchar 0) p ⊣⊢ emp.
 Proof. intros.
-  apply pred_ext.
+  apply bi.equiv_entails_2.
   apply data_at__tuchar_zero_array_inv.
   apply data_at__tuchar_zero_array; trivial.
 Qed. 
 
-Lemma data_at__tschar_zero_array_eq {cs} sh p (H: isptr p):
-  @data_at_ cs sh (tarray tschar 0) p = emp.  
+Lemma data_at__tschar_zero_array_eq {cs : compspecs} sh p (H: isptr p):
+  data_at_ sh (tarray tschar 0) p ⊣⊢ emp.
 Proof. intros.
-  apply pred_ext.
+  apply bi.equiv_entails_2.
   apply data_at__tschar_zero_array_inv.
   apply data_at__tschar_zero_array; trivial.
 Qed. 
 
 Lemma split2_data_at__Tarray_tuchar
-     : forall {cs} (sh : Share.t)  (n n1 : Z) (p : val),
+     : forall {cs : compspecs} (sh : Share.t)  (n n1 : Z) (p : val),
        0 <= n1 <= n -> isptr p ->field_compatible (Tarray tuchar n noattr) [] p ->
-       @data_at_ cs sh (Tarray tuchar n noattr) p =
-       @data_at_ cs sh (Tarray tuchar n1 noattr) p *
-       @data_at_ cs sh (Tarray tuchar (n - n1) noattr)
+       data_at_ sh (Tarray tuchar n noattr) p ⊣⊢
+       data_at_ sh (Tarray tuchar n1 noattr) p ∗
+       data_at_ sh (Tarray tuchar (n - n1) noattr)
          (field_address0 (Tarray tuchar n noattr) [ArraySubsc n1] p).
-Proof. intros. unfold data_at_ at 1; unfold field_at_.
+Proof.
+intros. unfold data_at_ at 1; unfold field_at_.
 rewrite field_at_data_at.
 erewrite (@split2_data_at_Tarray cs sh tuchar n n1).
 instantiate (1:= Zrepeat Vundef (n-n1)).
@@ -892,11 +895,11 @@ unfold default_val. simpl. autorewrite with sublist. reflexivity.
 Qed. 
 
 Lemma split2_data_at__Tarray_tschar
-     : forall {cs} (sh : Share.t)  (n n1 : Z) (p : val),
+     : forall {cs : compspecs} (sh : Share.t)  (n n1 : Z) (p : val),
        0 <= n1 <= n -> isptr p ->field_compatible (Tarray tschar n noattr) [] p ->
-       @data_at_ cs sh (Tarray tschar n noattr) p =
-       @data_at_ cs sh (Tarray tschar n1 noattr) p *
-       @data_at_ cs sh (Tarray tschar (n - n1) noattr)
+       data_at_ sh (Tarray tschar n noattr) p ⊣⊢
+       data_at_ sh (Tarray tschar n1 noattr) p ∗
+       data_at_ sh (Tarray tschar (n - n1) noattr)
          (field_address0 (Tarray tschar n noattr) [ArraySubsc n1] p).
 Proof. intros. unfold data_at_ at 1; unfold field_at_.
 rewrite field_at_data_at.
@@ -920,8 +923,8 @@ Lemma split2_data_at_Tarray_app:
                            (v1 v2: list (reptype t)) p,
     Zlength v1 = mid ->
     Zlength v2 = n-mid ->
-    data_at sh (tarray t n) (v1 ++ v2) p =
-    data_at sh (tarray t mid) v1  p *
+    data_at sh (tarray t n) (v1 ++ v2) p ⊣⊢
+    data_at sh (tarray t mid) v1  p ∗
     data_at sh (tarray t (n-mid)) v2
             (field_address0 (tarray t n) [ArraySubsc mid] p).
 Proof.
@@ -940,15 +943,15 @@ Qed.
 Fixpoint sepconN N (P: val -> mpred) sz (p:val):mpred :=
   match N with
     O => emp
-  | S n => (P p * sepconN n P sz (offset_val sz p))%logic
+  | S n => P p ∗ sepconN n P sz (offset_val sz p)
   end.
 
 Lemma mapsto_zeros_mapsto_nullval_N {cenv} N sh t b z:
        readable_share sh ->
        (align_chunk Mptr | Ptrofs.unsigned z) ->
        mapsto_zeros (Z.of_nat N * size_chunk Mptr) sh (Vptr b z)
-       |-- !! (0 <= Ptrofs.unsigned z /\
-               (Z.of_nat N * size_chunk Mptr + Ptrofs.unsigned z < Ptrofs.modulus)%Z) &&
+       ⊢ ⌜0 <= Ptrofs.unsigned z /\
+               (Z.of_nat N * size_chunk Mptr + Ptrofs.unsigned z < Ptrofs.modulus)%Z⌝ ∧
            sepconN N (fun p => mapsto sh (Tpointer t noattr) p nullval)
                      (@sizeof cenv (Tpointer t noattr)) (Vptr b z).
 Proof.
@@ -960,8 +963,8 @@ Proof. rewrite size_chunk_Mptr. unfold Ptrofs.max_unsigned.
  specialize Ptrofs.modulus_eq64.
  specialize Ptrofs.modulus_eq32.
  destruct (Archi.ptr64); intros X Y.
- rewrite Y; [ simpl; lia | trivial].
- rewrite X; [ simpl; lia | trivial].
+ rewrite Y; [ simpl; rep_lia | trivial].
+ rewrite X; [ simpl; rep_lia | trivial].
 Qed.
 
 Lemma sizeof_Tpointer cenv t a: @sizeof cenv (Tpointer t a) = if Archi.ptr64 then 8 else 4.
@@ -980,7 +983,7 @@ Lemma sepconN_mapsto_array {cenv t b sh} K : forall z
     (Hz: 0 <= Ptrofs.unsigned z /\
                Z.of_nat K * size_chunk Mptr + Ptrofs.unsigned z < Ptrofs.modulus),
     sepconN K (fun p : val => mapsto sh (Tpointer t noattr) p nullval) (size_chunk Mptr) (Vptr b z)
-|-- @data_at cenv sh (tarray (Tpointer t noattr) (Z.of_nat K)) (repeat nullval K) (Vptr b z).
+⊢ data_at sh (tarray (Tpointer t noattr) (Z.of_nat K)) (repeat nullval K) (Vptr b z).
 Proof.
   specialize (Zle_0_nat K); specialize size_chunk_range; intros SZ Kpos.
   induction K; intros.
@@ -991,7 +994,7 @@ Proof.
   replace (Z.of_nat (S K) * size_chunk Mptr)%Z with 
           (Z.of_nat K * size_chunk Mptr + size_chunk Mptr)%Z in Hz by lia.
   replace  (Z.of_nat (S K) - 1) with (Z.of_nat K) by lia.
-  eapply sepcon_derives.
+  eapply bi.sep_mono.
   - erewrite mapsto_data_at'; simpl; trivial.
     erewrite data_at_singleton_array_eq. apply derives_refl. trivial.
     red; simpl. rewrite sizeof_Tpointer. intuition. unfold size_chunk, Mptr in H2. destruct (Archi.ptr64); simpl; lia.
@@ -1003,15 +1006,15 @@ Proof.
       assert (c < Ptrofs.modulus).
       + eapply Z.le_lt_trans. 2: apply Hz. apply (Z.add_le_mono 0). apply Zmult_gt_0_le_0_compat; lia. lia.
       + lia. }
-    fold sepconN. unfold offset_val. eapply derives_trans.
+    fold sepconN. unfold offset_val. etrans.
     * apply IHK; clear IHK; trivial.
       ++ rewrite Ptrofs.add_unsigned. rewrite (Ptrofs.unsigned_repr (size_chunk Mptr)) by lia.
          rewrite Ptrofs.unsigned_repr by trivial.
          apply Z.divide_add_r; trivial. apply align_size_chunk_divides.
       ++ rewrite Ptrofs.add_unsigned. rewrite (Ptrofs.unsigned_repr (size_chunk Mptr)) by lia.
          rewrite Ptrofs.unsigned_repr by trivial. lia.
-    * apply derives_refl'. simpl. clear IHK.
-      f_equal. rewrite Zpos_P_of_succ_nat, <- Nat2Z.inj_succ. unfold field_address0.
+    * apply bi.equiv_entails_1_1. simpl. clear IHK.
+      f_equiv; hnf. unfold field_address0.
       rewrite if_true. reflexivity.
       red; repeat split; try solve [simpl; trivial; lia].
       ++ red. unfold tarray. rewrite sizeof_Tarray, sizeof_Tpointer, Z.max_r by lia.
@@ -1028,15 +1031,14 @@ Lemma mapsto_zeros_data_atTarrayTptr_nullval_N {cenv} N sh t b z:
        readable_share sh ->
        (align_chunk Mptr | Ptrofs.unsigned z) ->
        mapsto_zeros (Z.of_nat N * size_chunk Mptr) sh (Vptr b z)
-       |-- @data_at cenv sh (tarray (Tpointer t noattr) (Z.of_nat N)) (repeat nullval N) (Vptr b z).
-Proof. intros. 
-  eapply derives_trans.
-  eapply (mapsto_zeros_mapsto_nullval_N N sh); trivial.
+       ⊢ data_at sh (tarray (Tpointer t noattr) (Z.of_nat N)) (repeat nullval N) (Vptr b z).
+Proof. intros.
+  rewrite mapsto_zeros_mapsto_nullval_N; try done.
   Intros. apply sepconN_mapsto_array; trivial.
 Qed.
 
-Lemma mapsto_zeros_isptr z sh p : mapsto_zeros z sh p |-- !! isptr p.
-Proof. unfold mapsto_zeros. destruct p; try apply FF_left. apply prop_right. simpl; trivial. Qed.
+Lemma mapsto_zeros_isptr z sh p : mapsto_zeros z sh p ⊢ ⌜isptr p⌝.
+Proof. unfold mapsto_zeros. destruct p; try iIntros "[]". apply bi.pure_intro. simpl; trivial. Qed.
 
 Lemma field_compatible_byvalue {cs: compspecs}:
  forall big b small s gfs p k,
@@ -1131,34 +1133,11 @@ apply Zmult_le_compat_r; [ | lia].
 lia.
 Qed.
 
-#[export] Hint Extern 2 (field_compatible _ _ _) =>
-  (eapply field_compatible_byvalue0; [ reflexivity | eassumption | reflexivity..]) : field_compatible.
-#[export] Hint Extern 2 (field_compatible _ _ (offset_val _ _)) =>
-  (eapply field_compatible_byvalue'; [ reflexivity | eassumption | reflexivity..]) : field_compatible.
-
-#[export] Hint Extern 2 (field_address _ _ _ = field_address _ _ _) =>
-  (do 2 rewrite field_address_offset by auto with field_compatible;
-   reflexivity) : field_compatible.
-
-#[export] Hint Extern 2 (field_address _ _ _ = field_address0 _ _ _) =>
-  (rewrite field_address_offset by auto with field_compatible;
-   rewrite field_address0_offset by auto with field_compatible;
-   reflexivity) : field_compatible.
-
-#[export] Hint Extern 2 (field_address0 _ _ _ = field_address _ _ _) =>
-  (rewrite field_address_offset by auto with field_compatible;
-   rewrite field_address0_offset by auto with field_compatible;
-   reflexivity) : field_compatible.
-
-#[export] Hint Extern 2 (field_address0 _ _ _ = field_address0 _ _ _) =>
-  (do 2 rewrite field_address0_offset by auto with field_compatible;
-   reflexivity) : field_compatible.
-
 Lemma split2_data_at__Tarray_app {cs: compspecs}
      : forall (mid n : Z) (sh : Share.t) (t : type) (p : val),
        0 <= mid <= n ->
-       data_at_ sh (tarray t n) p = data_at_ sh (tarray t mid) p
-                                                * data_at_ sh (tarray t (n - mid)) 
+       data_at_ sh (tarray t n) p ⊣⊢ data_at_ sh (tarray t mid) p
+                                                ∗ data_at_ sh (tarray t (n - mid)) 
                                                     (field_address0 (tarray t n) (SUB mid) p).
 Proof.
 intros.
@@ -1166,12 +1145,12 @@ unfold tarray.
 rewrite !data_at__Tarray.
 fold (tarray t n). fold (tarray t mid). fold (tarray t (n-mid)).
 rewrite <- split2_data_at_Tarray_app by list_solve.
-f_equal. rewrite Zrepeat_app by list_solve. f_equal. lia.
+f_equiv. rewrite Zrepeat_app by list_solve. f_equal. lia.
 Qed.
 
 Lemma data__at_singleton_array_eq:
   forall {cs : compspecs} (sh : Share.t) (t : type) (p : val), 
-  data_at_ sh (tarray t 1) p = data_at_ sh t p.
+  data_at_ sh (tarray t 1) p ⊣⊢ data_at_ sh t p.
 Proof.
 intros.
 apply data_at_singleton_array_eq.
@@ -1226,9 +1205,10 @@ rewrite Z.mul_add_distr_l in H2.
 rewrite <- (Ptrofs.repr_unsigned i0), ptrofs_add_repr.
 rewrite Ptrofs.unsigned_repr.
 unfold sizeof.
+rewrite Z.add_0_l.
 replace  (Ptrofs.unsigned i0 + (Ctypes.sizeof t * j) + Ctypes.sizeof t * i1)
  with   (Ptrofs.unsigned i0 + (Ctypes.sizeof t * i1 + Ctypes.sizeof t * j))
-  by lia; auto.
+  by rep_lia; auto.
 unfold sizeof.
 pose proof (Ctypes.sizeof_pos t).
 assert (0 <= Ctypes.sizeof t * j <= Ctypes.sizeof t * j + Ctypes.sizeof t * i1) by nia.
@@ -1247,4 +1227,27 @@ auto with field_compatible.
 Opaque sizeof.
 Qed.
 
+End mpred.
 
+#[export] Hint Extern 2 (field_compatible _ _ _) =>
+  (eapply field_compatible_byvalue0; [ reflexivity | eassumption | reflexivity..]) : field_compatible.
+#[export] Hint Extern 2 (field_compatible _ _ (offset_val _ _)) =>
+  (eapply field_compatible_byvalue'; [ reflexivity | eassumption | reflexivity..]) : field_compatible.
+
+#[export] Hint Extern 2 (field_address _ _ _ = field_address _ _ _) =>
+  (do 2 rewrite field_address_offset by auto with field_compatible;
+   reflexivity) : field_compatible.
+
+#[export] Hint Extern 2 (field_address _ _ _ = field_address0 _ _ _) =>
+  (rewrite field_address_offset by auto with field_compatible;
+   rewrite field_address0_offset by auto with field_compatible;
+   reflexivity) : field_compatible.
+
+#[export] Hint Extern 2 (field_address0 _ _ _ = field_address _ _ _) =>
+  (rewrite field_address_offset by auto with field_compatible;
+   rewrite field_address0_offset by auto with field_compatible;
+   reflexivity) : field_compatible.
+
+#[export] Hint Extern 2 (field_address0 _ _ _ = field_address0 _ _ _) =>
+  (do 2 rewrite field_address0_offset by auto with field_compatible;
+   reflexivity) : field_compatible.
